commit

Projects/NatSuccSub/Basic.lean
@@ -1,3 +1,50 @@
 import Projects.NatSuccSub.Defs
 
 namespace NatSuccSub
+
+@[simp]
+def exprId : Expr :=
+  .arg 0
+
+def defId : Def where
+  arity := 1
+  expr := exprId
+
+def progId : Prog where
+  defs := [defId]
+
+-----
+
+@[simp] theorem defs_progId : progId.defs = [defId] := rfl
+@[simp] theorem arity_defId : defId.arity = 1 := rfl
+@[simp] theorem expr_defId : defId.expr = exprId := rfl
+@[simp] theorem main_progId : progId.main = defId := rfl
+@[simp] theorem wf_exprId : exprId.WF progId 1 := by simp [Expr.WF]
+@[simp] theorem wf_defId : defId.WF progId := wf_exprId
+@[simp] theorem arity_zero_progId : progId.arity 0 = 1 := rfl
+@[simp] theorem expr_zero_progId : progId.expr 0 = exprId := rfl
+@[simp] theorem Expr.eval_arg {i prog f args} : (arg i).eval prog f args = args[i]! := rfl
+@[simp] theorem Prog.defs_mk {ds} : defs ⟨ds⟩ = ds := rfl
+@[simp] theorem Prog.arity_zero {prog : Prog} : prog.arity 0 = 1 := rfl
+@[simp] theorem Prog.arity_one {prog : Prog} : prog.arity 1 = 2 := rfl
+
+@[simp, instance]
+theorem wf_progId : progId.WF := by
+  constructor; iterate 3 simp
+  intro F G hf hg; rcases hf with ⟨h₁, h₂, h₃⟩
+  rcases hg with ⟨h₄, h₅, h₆⟩; simp_all
+  rw [List.length_eq_one_iff] at h₁ h₄
+  obtain ⟨f, rfl⟩ := h₁; obtain ⟨g, rfl⟩ := h₄
+  simp_all; grind
+
+-- #check 0 #exit
+
+-- example : ¬(⟨[⟨1, .call 2 (λ n => if n ≠ 0 then default else .arg 0)⟩]⟩ : Prog).WF := by
+--   rintro ⟨-, -, -, h⟩
+--   contrapose! h; clear h
+--   use [λ (xs : List ℕ) => if xs.length ≠ 1 then default else 0]
+--   use [λ (xs : List ℕ) => if xs.length ≠ 1 then default else 1]
+--   simp
+--   split_ands
+--   ·
+--     constructor <;> simp
