Projects/NatSuccSub/Defs.lean
@@ -16,6 +16,7 @@ deriving Inhabited
 @[ext]
 structure Prog : Type where
   defs : List Def
+deriving Inhabited
 
 -----
 
@@ -45,6 +46,9 @@ def Prog.HasDef (prog : Prog) (i : ℕ) : Prop :=
 def Prog.arity (prog : Prog) (i : ℕ) : ℕ :=
   prog.def i |>.arity
 
+def Prog.expr (prog : Prog) (i : ℕ) : Expr :=
+  prog.def i |>.expr
+
 def Expr.WF (prog : Prog) (arity : ℕ) (e : Expr) : Prop :=
   match e with
   | .arg i => i ≤ arity
@@ -55,7 +59,21 @@ def Expr.WF (prog : Prog) (arity : ℕ) (e : Expr) : Prop :=
 def Def.WF (prog : Prog) (d : Def) : Prop :=
   d.expr.WF prog d.arity
 
+def Expr.eval (e : Expr) (prog : Prog) (fs : List (List ℕ → ℕ)) (args : List ℕ) : ℕ :=
+  match e with
+  | .arg i => args[i]!
+  | .call i xs => fs[i]! # List.range (prog.arity i)
+    |>.map λ i => xs i |>.eval prog fs args
+
+structure Prog.Compatible (prog : Prog) (fs : List (List ℕ → ℕ)) : Prop where
+  length_fs : fs.length = prog.defs.length
+  eq_default_of_ne_arity ⦃i⦄ : i < prog.defs.length → ∀ ⦃xs : List ℕ⦄,
+    xs.length ≠ prog.arity i → fs[i]! xs = default
+  eval_eq ⦃i⦄ : i < prog.defs.length → ∀ ⦃xs : List ℕ⦄, xs.length = prog.arity i →
+    (prog.expr i).eval prog fs xs = fs[i]! xs
+
 class Prog.WF (prog : Prog) : Prop where
   defs_ne_nil : prog.defs ≠ []
   arity_main : prog.main.arity = 1
   wf_def ⦃d⦄ : d ∈ prog.defs → d.WF prog
+  eq_of_compatible ⦃f g⦄ : prog.Compatible f → prog.Compatible g → f = g
